SporkProofs/WFSemantics.lean
@@ -3,35 +3,45 @@ import SporkProofs.WFSyntax
 import SporkProofs.Semantics
 import SporkProofs.IVec
 import SporkProofs.HeadIs
+import SporkProofs.SimpSet
 
-namespace StackFrameCode
-  inductive WF (fsigs B bsig ret) : StackFrameCode -> Prop
-    | code {c} : c.WF fsigs B bsig -> (code c).WF fsigs B bsig ret
-    | cont {b} : b.WFRets B bsig ret -> (cont b).WF fsigs B bsig ret
+theorem argswf (Γ : Scope) : IVec (Γ ⊢ · WF-var) ((List.range Γ).map Var.mk) :=
+  let rec h : (Γ : Scope) -> (n : Nat) ->
+              IVec ((Γ + n) ⊢ · WF-var) ((List.range' n Γ).map Var.mk)
+    | 0, n => .nil
+    | Γ + 1, n => .cons ⟨by simp⟩ (Nat.add_assoc Γ 1 n ▸
+                                   Nat.add_comm 1 n ▸
+                                   h Γ (n + 1))
+  List.range_eq_range' ▸ h Γ 0
 
-  namespace WF
-    notation (name := notationwf) fsigs:arg " ; " B:arg " ; " bsig:arg " ; " ret:arg " ⊢ " c:arg " WF-sfc" => WF fsigs B bsig ret c
+-- namespace StackFrameCode
+--   inductive WF (fsigs B bsig ret) : StackFrameCode -> Prop
+--     | code {c} : c.WF fsigs B bsig -> (code c).WF fsigs B bsig ret
+--     | cont {b} : b.WFRets B bsig ret -> (cont b).WF fsigs B bsig ret
 
-    instance {fsigs B bsig ret} : (c : StackFrameCode) ->
-             Decidable (fsigs; B; bsig; ret ⊢ c WF-sfc)
-      | .code c =>
-        decidable_of_iff (fsigs; B; bsig ⊢ c WF-code)
-          ⟨code, λ (code p) => p⟩
-      | .cont b =>
-        decidable_of_iff (B; bsig ⊢ b(ret) WF-cont)
-          ⟨cont, λ (cont p) => p⟩
+--   namespace WF
+--     notation (name := notationwf) fsigs:arg "; " B:arg "; " bsig:arg "; " ret:arg " ⊢ " c:arg " WF-sfc" => WF fsigs B bsig ret c
 
-    theorem c {fsigs B bsig ret c} :
-             fsigs; B; bsig; ret ⊢ (.code c) WF-sfc ->
-             fsigs; B; bsig ⊢ c WF-code
-      | code c => c
+--     instance {fsigs B bsig ret} : (c : StackFrameCode) ->
+--              Decidable (fsigs; B; bsig; ret ⊢ c WF-sfc)
+--       | .code c =>
+--         decidable_of_iff (fsigs; B; bsig ⊢ c WF-code)
+--           ⟨code, λ (code p) => p⟩
+--       | .cont b =>
+--         decidable_of_iff (B; bsig ⊢ b(ret) WF-cont)
+--           ⟨cont, λ (cont p) => p⟩
 
-    theorem b {fsigs B bsig b ret} :
-             fsigs; B; bsig; ret ⊢ (.cont b) WF-sfc ->
-             B; bsig ⊢ b(ret) WF-cont
-      | cont b => b
-  end WF
-end StackFrameCode
+--     theorem c {fsigs B bsig ret c} :
+--              fsigs; B; bsig; ret ⊢ (.code c) WF-sfc ->
+--              fsigs; B; bsig ⊢ c WF-code
+--       | code c => c
+
+--     theorem b {fsigs B bsig b ret} :
+--              fsigs; B; bsig; ret ⊢ (.cont b) WF-sfc ->
+--              B; bsig ⊢ b(ret) WF-cont
+--       | cont b => b
+--   end WF
+-- end StackFrameCode
 
 /-
   inductive WF (B : BlockSigs) (bsig : BlockSig) (b : Cont) : Prop where
@@ -44,25 +54,36 @@ namespace SpawnBlock
   inductive WF (B : BlockSigs) (bspwn : SpawnBlock) : Prop where
     | mk (_ : bspwn.b < B.length)
          (_ : B[bspwn.b].Γ = bspwn.args.length)
-         (_ : B[bspwn.b].σ.isExit)
+         (_ : B[bspwn.b].σ = [])
 
   namespace WF
-    notation (name := notationwf) B:arg " ⊢ " bspwn:arg " WF-spawn" => WF B bspwn
+    notation (name := notationwf) B:arg " ⊢ " bspwn " WF-spawn" => WF B bspwn
     
     instance {B: BlockSigs} (bspwn: SpawnBlock): Decidable (B ⊢ bspwn WF-spawn) :=
-      decidable_of_iff (∃ _ :bspwn.b < B.length,
+      decidable_of_iff (∃ _ : bspwn.b < B.length,
                         B[bspwn.b].Γ = bspwn.args.length ∧
-                        B[bspwn.b].σ.isExit)
+                        B[bspwn.b].σ = [])
         ⟨λ ⟨a, b, c⟩ => .mk a b c, λ | .mk a b c => ⟨a, b, c⟩⟩
 
     theorem b {B bspwn}: B ⊢ bspwn WF-spawn -> bspwn.b < B.length
-      | mk b _args _ex => b
+      | mk b _args _σ => b
+    theorem b' {F : Func} {bspwn} (wf : F.B ⊢ bspwn WF-spawn) : bspwn.b < F.size :=
+      F.size_eq_B_length ▸ wf.b
     theorem args {B bspwn}: (wf : B ⊢ bspwn WF-spawn) -> (B[bspwn.b]'(b wf)).Γ = bspwn.args.length
-      | mk _b args _ex => args
-    theorem isExit {B bspwn}: (wf : B ⊢ bspwn WF-spawn) -> (B[bspwn.b]'(b wf)).σ.isExit
-      | mk _b _args ex => ex
-    abbrev getExit {B bspwn} (wf: B ⊢ bspwn WF-spawn): Nat :=
-      (B[bspwn.b]'(b wf)).σ.getExit wf.isExit
+      | mk _b args _σ => args
+    theorem σ {B bspwn}: (wf : B ⊢ bspwn WF-spawn) -> (B[bspwn.b]'(b wf)).σ = []
+      | mk _b _args σ => σ
+
+    theorem init {P} (Pwf : P WF-program) : (P[0]'Pwf.main.zero_lt).B ⊢ .init WF-spawn :=
+      by let zlt := Pwf.main.zero_lt
+         let mainΓ := congrArg FuncSig.arity Pwf.main.get0eq
+         let entryΓ := congrArg BlockSig.Γ Pwf⁅0⁆.head.get0eq
+         simp only [getters] at mainΓ entryΓ
+         apply SpawnBlock.WF.mk <;> try (simp only [getters])
+         · let mainΓ : P[0].fsig.arity = 0 := mainΓ
+           simpa[mainΓ] using entryΓ
+         · simpa using congrArg BlockSig.σ Pwf⁅0⁆.head.get0eq
+         · exact Pwf⁅0⁆.head.zero_lt_map
   end WF
 end SpawnBlock
 
@@ -83,7 +104,7 @@ namespace SpawnDeque
     | mk (_ : IVec (B ⊢ · WF-spawn) ρ.unpr) (_: SpawnOrder canProm ρ.prom)
 
   namespace WF
-    notation (name := notationwf) B:arg " ; " canProm:arg " ⊢ " ρ:arg " WF-deque" => WF B canProm ρ
+    notation (name := notationwf) B:arg "; " canProm:arg " ⊢ " ρ:arg " WF-deque" => WF B canProm ρ
   
     instance {B canProm} : (ρ : SpawnDeque) -> Decidable (B; canProm ⊢ ρ WF-deque)
       | .mk u p => decidable_of_iff
@@ -141,294 +162,462 @@ namespace SpawnDeque
 end SpawnDeque
 
 namespace StackFrame
-  inductive WF (P : Program) (curr : Option Nat) (K : CallStack) (σ : Oblg) :
-               StackFrame -> Prop where
-    | mk {f ρ X c} :
-         (_ : f < P.size) ->
-         (σ : Oblg) ->
-         ρ.sig P[f].B = σ.sig ->
-         ρ.WF P[f].B K.allPromoted ->
-         (if curr.isNone then c.isCode else c.isCont) = true ->
-         c.WF P P[f].B ⟨X.length, σ⟩
-                (curr.elim P[f].fsig.ret id) ->
-         (mk f ρ X c).WF P curr K
+  inductive WF (P : Program) (K : CallStack) (gets : Nat) : StackFrame -> Prop where
+    | mk {f ρ X b} :
+         (flt : f < P.size) ->
+         (blt : b < P[f].B.length) ->
+         (P[f].B[b].Γ ≤ X.length + gets ∧ P[f].B[b].σ = ρ.sig P[f].B) ->
+         --P[f].B[b] = ⟨X.length + gets, P[f].B[b].r, ρ.sig P[f].B⟩ ->
+         P[f].B; K.allPromoted ⊢ ρ WF-deque ->
+         (mk f ρ X b).WF P K gets
 
   namespace WF
-    instance {P curr K} : (k : StackFrame) -> Decidable (k.WF P curr K)
-      | .mk f ρ X c =>
-        decidable_of_iff (∃ _ : f < P.size,
-                          
-                          ρ.WF P[f].B K.allPromoted ∧
-                          (if curr.isNone then c.isCode else c.isCont) = true ∧
-                          c.WF P.fsigs P[f].B ⟨X.length, ρ.sig⟩
-                            (curr.elim P[f].fsig.ret id))
+    notation (name := notationwf) P:arg "; " K:arg "; " gets:arg " ⊢ " k " WF-frame" => WF P K gets k
+    notation (name := notationwf') P:arg "; " K:arg " ⊢ " k " WF-frame" => WF P K 0 k
+    instance {P K gets} : (k : StackFrame) -> Decidable (P; K; gets ⊢ k WF-frame)
+      | .mk f ρ X b =>
+        decidable_of_iff (∃ flt : f < P.size,
+                          ∃ blt : b < P[f].B.length,
+                          --P[f].B[b] = ⟨X.length + gets, P[f].B[b].r, ρ.sig P[f].B⟩ ∧
+                          (P[f].B[b].Γ ≤ X.length + gets ∧ P[f].B[b].σ = ρ.sig P[f].B) ∧
+                          P[f].B; K.allPromoted ⊢ ρ WF-deque)
           ⟨λ ⟨a, b, c, d⟩ => ⟨a, b, c, d⟩, λ ⟨a, b, c, d⟩ => ⟨a, b, c, d⟩⟩
 
-    theorem flt {P curr canProm} : {k : StackFrame} ->
-                k.WF P curr canProm -> k.f < P.size
-      | .mk _f _ρ _X _c, mk flt _ρwf _cwf _cb => flt
-  end WF
+    theorem flt {P K gets} : {k : StackFrame} ->
+                P; K; gets ⊢ k WF-frame -> k.f < P.size
+      | .mk _f _ρ _X _b, mk flt _blt _bsig _ρwf => flt
 
-  @[simp] def func {P curr canProm} (k : StackFrame) (kwf : k.WF P curr canProm) : Func :=
-    P[k.f]'kwf.flt
+    theorem blt {P K gets} : {k : StackFrame} ->
+                (wf : P; K; gets ⊢ k WF-frame) -> k.b < (P[k.f]'wf.flt).B.length
+      | .mk _f _ρ _X _b, mk _flt blt _bsig _ρwf => blt
 
-  namespace WF
+    theorem blt' {P K gets k} (wf : P; K; gets ⊢ k WF-frame) :
+                 k.b < (P[k.f]'wf.flt).size :=
+      (P[k.f]'wf.flt).size_eq_B_length ▸ wf.blt
 
-    theorem ρwf {P curr canProm} : {k : StackFrame} ->
-                k.WF P curr canProm -> k.ρ.WF P.fsigs canProm
-      | .mk _f _ρ _X _c, mk _flt ρwf _cwf _cb => ρwf
-    theorem cwf {P curr canProm} : {k : StackFrame} -> (kwf : k.WF P curr canProm) ->
-                k.c.WF P.fsigs (k.func kwf).B k.bsig
-                         (curr.elim (k.func kwf).fsig.ret id)
-      | .mk _f _ρ _X _c, mk _flt _ρwf _cb cwf => cwf
-    theorem cwf' {P curr canProm} : {k : StackFrame} -> (kwf : k.WF P curr canProm) ->
-                 k.c.WF P.fsigs P[k.f]!.B k.bsig
-                          (curr.elim P[k.f]!.fsig.ret id)
-      | .mk f _ρ _X _c, mk flt _ρwf _cb cwf =>
-        getElem!_pos P f flt ▸ cwf
-    theorem cwf'' {P curr canProm} : {k : StackFrame} -> (kwf : k.WF P curr canProm) ->
-                  let flt : k.f < P.size := kwf.flt
-                  k.c.WF P.fsigs P[k.f].B k.bsig
-                           (curr.elim P[k.f].fsig.ret id)
-      | .mk _f _ρ _X _c, mk _flt _ρwf _cb cwf => cwf
-    theorem cb {P curr canProm} : {k : StackFrame} -> (kwf : k.WF P curr canProm) ->
-               (if curr.isNone then k.c.isCode else k.c.isCont) = true
-      | .mk _f _ρ _X _c, mk _flt _ρwf cb _cwf => cb
-    theorem isCode {P canProm} : {k : StackFrame} ->
-                   (kwf : k.WF P none canProm) -> k.c.isCode := cb
-    theorem isCont {P canProm ret} : {k : StackFrame} ->
-                   (kwf : k.WF P (some ret) canProm) -> k.c.isCont := cb
+    theorem ρwf {P K gets} : {k : StackFrame} ->
+                (wf : P; K; gets ⊢ k WF-frame) -> (P[k.f]'wf.flt).B; K.allPromoted ⊢ k.ρ WF-deque
+      | .mk _f _ρ _X _b, mk _flt _blt _bsig ρwf => ρwf
 
-    theorem castCanProm {P curr canProm} : {k : StackFrame} ->
-                        (canProm' : Bool) -> canProm ≤ canProm' ->
-                        (kwf : k.WF P curr canProm) -> k.WF P curr canProm'
-      | .mk _f _ρ _X _c, canProm', l, .mk flt ρwf cwf cb =>
-        .mk flt (ρwf.castCanProm canProm' l) cwf cb
+    theorem bsig {P K gets} : {k : StackFrame} ->
+                 (wf : P; K; gets ⊢ k WF-frame) ->
+                 (((P[k.f]'wf.flt).B[k.b]'wf.blt).Γ ≤ k.X.length + gets ∧
+                  ((P[k.f]'wf.flt).B[k.b]'wf.blt).σ = k.ρ.sig (P[k.f]'wf.flt).B)
+                 -- ((P[k.f]'wf.flt).B[k.b]'wf.blt) = ⟨k.X.length + gets, ((P[k.f]'wf.flt).B[k.b]'wf.blt).r, k.ρ.sig (P[k.f]'wf.flt).B⟩
+      | .mk _f _ρ _X _b, mk _flt _blt bsig _ρwf => bsig
 
-    theorem entry
-        {P} (Pwf : P.WF) {f canProm} {X : List Val}
-        (p : f < P.size)
-        (sigwf : P[f].fsig.arity = X.length) :
-        WF P none canProm ⟨f, ∅, X, .codeEntry P f⟩ :=
-      let fwf := Pwf.1.get ⟨f, p⟩
-      let c' : Code.WF P.fsigs P[f].B P[f].fsig.ret
-                ⟨X.length, []⟩ P[f]!.blocks.head!.code :=
-        sigwf ▸
-        Eq.symm (getElem!_pos P f p) ▸
-        fwf.2.headeq ▸
-        fwf.2.head!eq ▸
-        (fwf.1.head fwf.2.nonnil).1
-      ⟨p, SpawnDeque.WF.empty, rfl, .code c'⟩
+    theorem bsig! {P K gets} : {k : StackFrame} ->
+                 (wf : P; K; gets ⊢ k WF-frame) ->
+                 (P[k.f]!.B[k.b]!.Γ ≤ k.X.length + gets ∧
+                  P[k.f]!.B[k.b]!.σ = k.ρ.sig P[k.f]!.B)
+--                 P[k.f]!.B[k.b]! = ⟨k.X.length + gets, P[k.f]!.B[k.b]!.r, k.ρ.sig P[k.f]!.B⟩
+      | .mk f _ρ _X b, mk flt blt bsig _ρwf =>
+        getElem!_pos P f flt ▸
+        getElem!_pos P[f].B b blt ▸
+        bsig
+
+    theorem changeStack {P K K' gets k} :
+                        P; K; gets ⊢ k WF-frame ->
+                        (K.allPromoted ≤ K'.allPromoted) ->
+                        P; K'; gets ⊢ k WF-frame
+      | .mk flt blt bsig ρwf, klt =>
+        .mk flt blt bsig (ρwf.castCanProm K'.allPromoted klt)
+
+    theorem spawn {P f bspwn} (flt : f < P.size) (bwf : P[f].B ⊢ bspwn WF-spawn) :
+                  P; .nil ⊢ .spawn f bspwn WF-frame :=
+      let blt := bwf.b
+      -- let sigeq : P[f].B[bspwn.b] = ⟨bspwn.args.length, P[f].B[bspwn.b].r, []⟩ :=
+      --   bwf.args ▸ bwf.σ ▸ rfl
+      ⟨flt, blt, ⟨bwf.args ▸ Nat.le_refl P[f].B[bspwn.b].Γ, bwf.σ⟩, .empty⟩
+
+    theorem entry {P} (Pwf : P WF-program) {f K X} (flt : f < P.size)
+                  (sigwf : P[f].fsig.arity = X.length) : P; K ⊢ ⟨f, ∅, X, 0⟩ WF-frame :=
+      let blt : 0 < P[f].B.length :=
+        Pwf⁅f⁆.head.zero_lt_map
+--      let sigeq := sigwf ▸ Pwf⁅f⁆.head.get0eq_map ▸ rfl
+      ⟨flt, blt, ⟨sigwf ▸ Pwf⁅f⁆.head.get0eq_map ▸ by simp,
+                  List.getElem_map Block.bsig ▸
+                  congrArg (·.σ) Pwf⁅f⁆.head.get0eq⟩, .empty⟩
 
     theorem goto_rets
-        {P} (Pwf : P.WF) {f canProm ρ} {X Y : ValMap} {bnext} {y : List Var}
-        (p : f < P.size)
-        (ρwf : ρ.WF P.fsigs canProm)
-        (bnext_wf : bnext.WFRets P[f].B ⟨X.length, ρ.sig⟩ y.length)
-        (y_wf : IVec (·.WF Y.length) y) :
-        StackFrame.WF P none canProm
-          ⟨f, ρ, X[bnext.args]! ++ Y[y]!, .codeOf P f bnext⟩ :=
-      let ⟨bwf, sigwf, x_wf⟩ := bnext_wf
-      let bwf' : bnext.b < P[f].size :=
-        by simp; exact (List.length_map Block.bsig ▸ bwf)
-      let xlen : bnext.args.length = X[bnext.args].length :=
-        x_wf.map_length (λ x xwf => X[x])
-      let ylen : y.length = Y[y].length :=
-        y_wf.map_length (λ y ywf => Y[y])
-      let code_wf : P[f]![bnext.b]!.code.WF
-                      P.fsigs P[f].B P[f].fsig.ret
-                      ⟨(X[bnext.args]! ++ Y[y]!).length, ρ.sig⟩ := by
-        rw[codeOfGetElem p bwf',
-           argsOfGetElem x_wf,
-           argsOfGetElem y_wf,
-           List.length_append,
-           ← xlen, ← ylen]
-        simp at sigwf
-        simp
-        rw[← sigwf];
-        exact ((Pwf.1.get ⟨f, p⟩).1.get ⟨bnext.b, bwf'⟩).1
-      ⟨p, ρwf, rfl, .code code_wf⟩
-  
+        {P} {f K ρ} {X : ValMap} {bnext : Cont} {r : Nat}
+        (flt : f < P.size)
+        (ρwf : P[f].B; K.allPromoted ⊢ ρ WF-deque)
+        (bnext_wf : P[f].B; ⟨X.length, P[f].B[bnext.b]!.r, ρ.sig P[f].B⟩ ⊢ bnext(r) WF-cont) :
+        P; K; r ⊢ ⟨f, ρ, X[bnext.args]'bnext_wf.args, bnext.b⟩ WF-frame :=
+      ⟨flt,
+       bnext_wf.blt,
+       bnext_wf.bsig ▸ by simp; rw[ValMap.getElem_length bnext_wf.args]; simp,
+       --bnext_wf.bsig ▸ by simp; symm; exact ValMap.getElem_length bnext_wf.args,
+       ρwf⟩
+
     theorem goto
-        {P} (Pwf : P.WF) {f canProm ρ} {X : ValMap} {bnext}
+        {P} {f K ρ} {X : ValMap} {bnext : Cont}
         (p : f < P.size)
-        (ρwf : ρ.WF P.fsigs canProm)
-        (bnext_wf : bnext.WF P[f].B ⟨X.length, ρ.sig⟩) :
-        StackFrame.WF P none canProm ⟨f, ρ, X[bnext.args]!, .codeOf P f bnext⟩ :=
-      List.append_nil X[bnext.args]! ▸
-      goto_rets Pwf (Y := []) (y := []) p ρwf bnext_wf.cast0 .nil
+        (ρwf : P[f].B; K.allPromoted ⊢ ρ WF-deque)
+        (bnext_wf : P[f].B; ⟨X.length, P[f].B[bnext.b]!.r, ρ.sig P[f].B⟩ ⊢ bnext WF-cont) :
+        P; K ⊢ ⟨f, ρ, X[bnext.args]'bnext_wf.args, bnext.b⟩ WF-frame :=
+      goto_rets p ρwf bnext_wf
   
     theorem goto_entry
-        {P} (Pwf : P.WF) {f canProm} {X : ValMap} {x : List Var}
+        {P} (Pwf : P WF-program) {f K} {X : ValMap} {x : List Var}
         (p : f < P.size)
         (xwf : IVec (·.WF X.length) x)
         (sigwf : P[f].fsig.arity = x.length) :
-        StackFrame.WF P none canProm ⟨f, ∅, X[x]!, .codeEntry P f⟩ :=
-      entry Pwf p (argsOfGetElem xwf ▸
-                    xwf.map_length (λ x xwf => X[x]) ▸
-                    sigwf)
-  
+        P; K ⊢ ⟨f, ∅, X[x]'xwf, 0⟩ WF-frame :=
+      entry Pwf p (xwf.map_length (λ x xwf => X[x]) ▸ sigwf)
+  end WF
+
+  @[simp] def ret {P K gets} (k : StackFrame) (kwf : P; K; gets ⊢ k WF-frame) : Nat :=
+    ((P[k.f]'kwf.flt).B[k.b]'kwf.blt).r
+
+  @[simp] def ret! (P : Program) (k : StackFrame) : Nat :=
+    P[k.f]!.B[k.b]!.r
+
+  @[simp] def code {P K gets} (k : StackFrame) (kwf : P; K; gets ⊢ k WF-frame) : Code :=
+    ((P[k.f]'kwf.flt)[k.b]'kwf.blt').code
+
+  namespace WF
+    @[simp] theorem ret!_eq_ret {P K k gets} (kwf : P; K; gets ⊢ k WF-frame) : k.ret! P = k.ret kwf :=
+      by rw[ret, ret!,
+            getElem!_pos P k.f kwf.flt,
+            getElem!_pos (P[k.f]'kwf.flt).B k.b kwf.blt]
+
+    @[simp] theorem code!_eq_code {P K k gets} (kwf : P; K; gets ⊢ k WF-frame) : k.code! P = k.code kwf :=
+      by rw[code, code!,
+            getElem!_pos P k.f kwf.flt,
+            getElem!_pos (P[k.f]'kwf.flt) k.b kwf.blt']
   end WF
 end StackFrame
 
 
 namespace CallStack
+
   /--
-  (Potentially partial) call stack.
-  When `get` is omitted (`none`), this must be a full call
-  stack, where the current frame has `code` rather than `cont`
-  When `get` is `some n`, it is a partial call stack awaiting
+  (Potentially partial) call stack, awaiting a return of `gets` args.
+  When `gets` is `none`, this must be a full call stack,
+  where the current frame is at the surface of the stack.
+  When `gets` is `some n`, it is a partial call stack awaiting
   a return of `n` args from the following stack frame
   -/
-  inductive WF (P : Program) : (get : Option Nat := none) -> CallStack -> Prop where
-    | nil {gets} : nil.WF P (some gets)
-    | cons {K k gets} :
-           (kwf : k.WF P gets K.allPromoted) ->
-           K.WF P (k.func kwf).fsig.ret ->
+  inductive WF (P : Program) : (gets : Option Nat) -> CallStack -> Prop where
+    | nil {gets : Nat} : nil.WF P (some gets)
+    | cons {K k} {gets : Option Nat} :
+           P; K; (gets.getD 0) ⊢ k WF-frame ->
+           K.WF P (some (k.ret! P)) ->
            (K ⬝ k).WF P gets
 
   namespace WF
     notation (name := callstackwfcons) t " ⬝wf " h:arg => WF.cons h t
+    notation (name := notationwf) P:arg "; " gets:arg " ⊢ " K:arg " WF-stack" => WF P gets K
+    notation (name := notationwf') P:arg " ⊢ " K " WF-stack" => WF P none K
 
     instance instDecidable {P} : {gets : Option Nat} -> (K : CallStack) ->
-                           Decidable (K.WF P gets)
-      | some gets, .nil => isTrue WF.nil
-      | none, .nil => isFalse (by cases ·)
+                           Decidable (P; gets ⊢ K WF-stack)
+      | some gets, .nil => isTrue .nil
+      | none, .nil => isFalse (λ _ => by contradiction)
       | gets, K ⬝ k =>
-        dite (k.WF P gets K.allPromoted)
-          (λ kwf => let Kwfdec : Decidable (K.WF P (some (k.func kwf).fsig.ret)) :=
-                      instDecidable K
-                    decidable_of_iff (K.WF P (some (k.func kwf).fsig.ret))
-                      ⟨cons kwf, λ | cons _kwf' Kwf => Kwf⟩)
-          (isFalse ∘ λ | kₙwf, cons kwf _Kwf => kₙwf kwf)
+        let _ : Decidable (P; (k.ret! P) ⊢ K WF-stack) := instDecidable K
+        decidable_of_iff (P; K; (gets.getD 0) ⊢ k WF-frame ∧ K.WF P (some (k.ret! P)))
+          ⟨λ ⟨a, b⟩ => .cons a b, λ | .cons a b => ⟨a, b⟩⟩
+        -- dite (P; K; (gets.getD 0) ⊢ k WF-frame)
+        --   (λ kwf => let _ : Decidable (P; (k.ret kwf) ⊢ K WF-stack) :=
+        --               instDecidable K
+        --             decidable_of_iff (P; (k.ret kwf) ⊢ K WF-stack)
+        --               ⟨cons kwf, λ | cons _kwf' Kwf => Kwf⟩)
+        --   (isFalse ∘ λ | kₙwf, cons kwf _Kwf => kₙwf kwf)
 
-    theorem nonnil {P} {K : CallStack} (Kwf : K.WF P none) : K ≠ CallStack.nil :=
+    theorem nonnil {P} {K : CallStack} (Kwf : P ⊢ K WF-stack) : K ≠ CallStack.nil :=
       by cases Kwf <;> simp
     theorem head' {P gets} :
                   {K : CallStack} ->
                   (nn : K ≠ CallStack.nil) ->
-                  K.WF P gets ->
-                  (K.head nn).WF P gets K.tail.allPromoted
+                  P; gets ⊢ K WF-stack ->
+                  P; K.tail; (gets.getD 0) ⊢ (K.head nn) WF-frame
       | _K ⬝ _k, _nn, _Kwf ⬝wf kwf => kwf
     theorem tail' {P gets} :
                   {K : CallStack} ->
                   (nn : K ≠ CallStack.nil) ->
-                  (Kwf : K.WF P gets) ->
-                  K.tail.WF P (some (P[(K.head nn).f]'(Kwf.head' nn).flt).fsig.ret)
+                  (Kwf : P; gets ⊢ K WF-stack) ->
+                  P; (some ((K.head nn).ret! P)) ⊢ K.tail WF-stack
       | _K ⬝ _k, _nn, Kwf ⬝wf _kwf => Kwf
+    theorem head! {P gets} :
+                  {K : CallStack} ->
+                  (nn : K ≠ CallStack.nil) ->
+                  P; gets ⊢ K WF-stack ->
+                  P; K.tail; (gets.getD 0) ⊢ K.head! WF-frame
+      | _K ⬝ _k, _nn, _Kwf ⬝wf kwf => kwf
 
-    theorem head {P gets K k} (Kwf : (K ⬝ k).WF P gets) :
-                 k.WF P gets K.allPromoted :=
+    theorem head {P gets K k} (Kwf : P; gets ⊢ (K ⬝ k) WF-stack) :
+                 P; K; (gets.getD 0) ⊢ k WF-frame :=
       head' (by simp) Kwf
 
-    theorem tail {P gets K k} (Kwf : (K ⬝ k).WF P gets) :
-                  K.WF P (some (P[k.f]'Kwf.head.flt).fsig.ret) :=
+    theorem tail {P gets K k} (Kwf : P; gets ⊢ (K ⬝ k) WF-stack) :
+                 P; (some (k.ret! P)) ⊢ K WF-stack :=
       tail' (by simp) Kwf
+
+    theorem current! {P K} (Kwf : P ⊢ K WF-stack) :
+                     P; K.tail ⊢ K.head! WF-frame :=
+      head! Kwf.nonnil Kwf
+
+    theorem current {P K} (Kwf : P ⊢ K WF-stack) :
+                    P; K.tail ⊢ (K.head Kwf.nonnil) WF-frame :=
+      head' Kwf.nonnil Kwf
   end WF
 
-  @[simp] def retjoin?! {P get} : (K : CallStack) -> K.WF P get -> Option Nat
-    | .nil, _wf => none
-    | .nil ⬝ k, wf => some (k.func wf.head).fsig.ret
-    | K ⬝ _k, wf => K.retjoin?! wf.tail
+  @[simp] def retjoin?! (P : Program) : (K : CallStack) -> Option Nat
+    | .nil => none
+    | .nil ⬝ k => some (k.ret! P)
+    | K ⬝ _k => K.retjoin?! P
   
-  theorem retjoin_eq_retjoin?! {P get} : {K : CallStack} -> (wf : K.WF P get) ->
-          (if K = .nil then none else some (K.retjoin P)) = K.retjoin?! wf
+  theorem retjoin_eq_retjoin?! {P get} : {K : CallStack} -> (wf : P; get ⊢ K WF-stack) ->
+          (if K = .nil then none else some (K.retjoin P)) = K.retjoin?! P
     | .nil, _wf =>
       rfl
-    | .nil ⬝ k, (_ ⬝wf kwf) =>
-      congrArg (α := Func) (λ x => some x.fsig.ret) (getElem!_pos P k.f kwf.flt)
+    | .nil ⬝ k, (_ ⬝wf kwf) => by
+      simp only [reduceCtorEq, if_false, retjoin?!, retjoin, StackFrame.ret!]
     | K ⬝ k ⬝ _k', wf =>
       retjoin_eq_retjoin?! (K := K ⬝ k) wf.tail
 
+  @[simp] def bsig! (P : Program) (K : CallStack) : BlockSig :=
+    ⟨K.head!.X.length,
+     (P[K.head!.f]!.B[K.head!.b]!).r,
+     K.head!.ρ.sig P[K.head!.f]!.B⟩
+  @[simp] def bsig {P : Program} (K : CallStack) (wf : P ⊢ K WF-stack) : BlockSig :=
+    let flt := wf.current.flt
+    let blt := wf.current.blt
+    ⟨(K.head wf.nonnil).X.length,
+     (P[(K.head wf.nonnil).f].B[(K.head wf.nonnil).b]).r,
+     (K.head wf.nonnil).ρ.sig P[(K.head wf.nonnil).f].B⟩
+  @[simp] def bsig' {P : Program} : (K : CallStack) -> (wf : P ⊢ K WF-stack) -> BlockSig
+    | K ⬝ ⟨f, ρ, X, b⟩, wf =>
+      let flt := wf.current.flt
+      let blt := wf.current.blt
+      ⟨X.length, P[f].B[b].r, ρ.sig P[f].B⟩
+  theorem bsig_eq_bsig' {P : Program} : {K : CallStack} -> (wf : P ⊢ K WF-stack) -> K.bsig wf = K.bsig' wf
+    | _K ⬝ ⟨_f, _ρ, _X, _b⟩, _wf => rfl
+  theorem bsig!_eq_bsig {P : Program} : {K : CallStack} -> (wf : P ⊢ K WF-stack) -> K.bsig wf = K.bsig! P
+    | _K ⬝ ⟨f, _ρ, _X, b⟩, wf =>
+      by simp only [bsig, getters, bsig!]
+         rw[getElem!_pos P f wf.current.flt,
+            getElem!_pos (P[f]'wf.current.flt).B b wf.current.blt]
+
+  -- @[simp] def code! (P : Program) (K : CallStack) : Code :=
+  --   K.head!.code! P
+  @[simp] def code {P : Program} (K : CallStack) (wf : P ⊢ K WF-stack) : Code :=
+    (K.head wf.nonnil).code wf.current
+
   namespace WF
     theorem append {P} : {K K' : CallStack} -> {gets : Option Nat} ->
-                   K.WF P (some (K'.retjoin P)) -> K'.WF P gets ->
-                   (gets.isNone ∨ K' ≠ .nil) -> K.allPromoted -> (K ++ K').WF P gets
-      | K, .nil ⬝ k, gets, Kwf, K'wf@(.nil ⬝wf kwf), _, kprom =>
+                   P; (some (K'.retjoin P)) ⊢ K WF-stack -> P; gets ⊢ K' WF-stack ->
+                   K' ≠ .nil -> K.allPromoted -> P; gets ⊢ (K ++ K') WF-stack
+      | K, .nil ⬝ k, gets, Kwf, K'wf@(.nil ⬝wf kwf), _knn, kprom =>
         by simp; exact
-          (Option.some_inj.mp (retjoin_eq_retjoin?! K'wf) ▸ Kwf) ⬝wf (kprom ▸ kwf)
+          (Option.some_inj.mp (retjoin_eq_retjoin?! K'wf) ▸ Kwf) ⬝wf
+          (kwf.changeStack (λ _ => kprom))
       | K, K' ⬝ k' ⬝ k, gets, Kwf, K'wf ⬝wf kwf, p, kprom =>
-        let kprom' := allPromoted_iff_nil.mp kprom
-        let kp : (K' ⬝ k').unpr = (K ++ (K' ⬝ k')).unpr :=
-          by simp; rw[kprom']
-        (append Kwf K'wf (Or.inr (by simp)) kprom) ⬝wf
-          (by simp at kwf; simp; rw[kprom']; exact kwf)
+        (append Kwf K'wf (λ x => by contradiction) kprom) ⬝wf
+          (kwf.changeStack (by simp[← ·, allPromoted_iff_nil.mp kprom]))
 
     theorem unappend {P} : {get : Option Nat} -> {K K' : CallStack} ->
-                     (K ++ K').WF P get -> (K' ≠ .nil) -> K.allPromoted ->
-                     K.WF P (some (K'.retjoin P)) ∧ K'.WF P get
+                     P; get ⊢ (K ++ K') WF-stack -> (K' ≠ .nil) -> K.allPromoted ->
+                     P; (some (K'.retjoin P)) ⊢ K WF-stack ∧ P; get ⊢ K' WF-stack
       | get, K, .nil ⬝ k, wf, _, kprom =>
-        let wf' : (K ⬝ k).WF P get :=
+        let wf' : P; get ⊢ (K ⬝ k) WF-stack :=
           by rw[@append_cons K .nil k] at wf; exact wf
-        let k_wf : k.WF P get true :=
-          kprom ▸ wf'.head
-        ⟨by simp only[retjoin]
-            rw[getElem!_pos P k.f k_wf.flt]
-            exact wf'.tail,
-         .nil ⬝wf k_wf⟩
+        let k_wf : P; K; (get.getD 0) ⊢ k WF-frame :=
+          wf'.head -- ⟨wf'.head.flt, wf'.head.blt, wf'.head.bsig, wf'.head.ρwf⟩
+          --⟨wf'.head.flt, kprom ▸ wf'.head.ρwf, wf'.head.cwf⟩
+        let nil_k_wf := .nil ⬝wf (k_wf.changeStack (K' := .nil) (λ _ => rfl))
+        let rr : some ((.nil ⬝ k).retjoin P) = (.nil ⬝ k).retjoin?! P :=
+          retjoin_eq_retjoin?! nil_k_wf
+        ⟨rr ▸ wf'.tail, nil_k_wf⟩
       | get, K, (K' ⬝ k') ⬝ k, wf, _, kprom =>
         let ⟨Kwf, K'wf⟩ := unappend wf.tail (by simp) kprom
         let kprom' := allPromoted_iff_nil.mp kprom
         let kp : [] ++ (K' ⬝ k').unpr = K.unpr ++ (K' ⬝ k').unpr :=
           kprom'.symm ▸ rfl
-        let k'wf : k.WF P get (K' ⬝ k').allPromoted := by
-          show k.WF P get ((K' ⬝ k').unpr = [])
-          rw[← List.nil_append (K' ⬝ k').unpr, kp, ← append_unpr]
-          exact wf.head
+        let k'wf : P; (K' ⬝ k'); (get.getD 0) ⊢ k WF-frame :=
+          wf.head.changeStack (λ kap => by simp at kap; simp[kap])
         ⟨Kwf, K'wf ⬝wf k'wf⟩
+
+    theorem code!_eq_code {P : Program} {K : CallStack} (Kwf : P ⊢ K WF-stack) : K.code! P = K.code Kwf :=
+      by rw[CallStack.code!,
+            CallStack.code,
+            CallStack.head!_eq_head,
+            Kwf.current.code!_eq_code]
+
+    theorem code {P : Program} (Pwf : P WF-program) :
+                 {K : CallStack} -> (Kwf : P ⊢ K WF-stack) ->
+                 P.fsigs; (P[(K.head Kwf.nonnil).f]'Kwf.current.flt).B; (K.bsig Kwf) ⊢
+                   (K.code Kwf) WF-code
+      | K ⬝ k, Kwf ⬝wf kwf =>
+        let flt := kwf.flt
+        let blt : k.b < P[k.f].size :=
+          by simpa using kwf.blt
+        let Xlen : (P[k.f].B[k.b]'kwf.blt).Γ ≤ k.X.length :=
+          by simpa only [Option.getD_none, Nat.add_zero] using kwf.bsig.1
+        by simp only [getters, CallStack.code, StackFrame.code, CallStack.bsig]
+           rw[← kwf.bsig.2,
+              ← Nat.add_sub_of_le Xlen]
+           simpa using Pwf⁅k.f⁆⁅k.b⁆.code.weaken_Γ
+
+    theorem code! {P : Program} (Pwf : P WF-program) {K : CallStack} (Kwf : P ⊢ K WF-stack) :
+                  P.fsigs; P[K.head!.f]!.B; (K.bsig! P) ⊢ (K.code! P) WF-code :=
+      K.head!_eq_head Kwf.nonnil ▸
+      getElem!_pos P (K.head Kwf.nonnil).f Kwf.current.flt ▸
+      code!_eq_code Kwf ▸
+      bsig!_eq_bsig Kwf ▸
+      code Pwf Kwf
+
+    theorem spawn {P : Program} {f : FuncIdx} {bspwn : SpawnBlock}
+                  (flt : f < P.size) (bwf : P[f].B ⊢ bspwn WF-spawn) :
+                  P ⊢ spawn f bspwn WF-stack :=
+      .nil ⬝wf (.spawn flt bwf)
   end WF
 end CallStack
 
+namespace Thread
+  inductive WF (P : Program) : Thread -> Prop where
+    | mk {K c} :
+         P ⊢ K WF-stack ->
+         P.fsigs; P[K.head!.f]!.B; (K.bsig! P) ⊢ c WF-code ->
+         WF P (K ⋄ c)
+
+  namespace WF
+    notation (name := notationwf) P:arg " ⊢ " T " WF-thread" => WF P T
+
+    theorem K {P} {T : Thread} : (wf : P ⊢ T WF-thread) -> P ⊢ T.K WF-stack
+      | .mk K _c => K
+    theorem c! {P} {T : Thread} : P ⊢ T WF-thread ->
+              P.fsigs; (P[T.K.head!.f]!).B; (T.K.bsig! P) ⊢ T.c WF-code
+      | .mk _K c => c
+    theorem c {P} {T : Thread} (wf : P ⊢ T WF-thread) :
+              P.fsigs; (P[(T.K.head wf.K.nonnil).f]'wf.K.current.flt).B; (T.K.bsig wf.K) ⊢ T.c WF-code :=
+      getElem!_pos P (T.K.head wf.K.nonnil).f wf.K.current.flt ▸
+      T.K.head!_eq_head wf.K.nonnil ▸
+      T.K.bsig!_eq_bsig wf.K ▸
+      wf.c!
+
+    theorem nonnil {P} {T : Thread} (wf : P ⊢ T WF-thread) : T.K ≠ .nil := wf.K.nonnil
+
+    instance {P} : {T : Thread} -> Decidable (P ⊢ T WF-thread)
+      | .nil ⋄ c => isFalse (λ p => by contradiction)
+      | K ⬝ k ⋄ c =>
+        decidable_of_iff (P ⊢ (K ⬝ k) WF-stack ∧
+                          P.fsigs; P[k.f]!.B; ((K ⬝ k).bsig! P) ⊢ c WF-code)
+          ⟨λ ⟨a, b⟩ => ⟨a, b⟩, λ ⟨a, b⟩ => ⟨a, b⟩⟩
+  end WF
+
+  @[simp] def fromStack {P : Program} (K : CallStack) (Kwf : P ⊢ K WF-stack) : Thread :=
+    K ⋄ K.code Kwf
+
+  @[simp] def spawn (P : Program) (f : FuncIdx) (bspwn : SpawnBlock)
+                    (flt : f < P.size) (bwf : P[f].B ⊢ bspwn WF-spawn) : Thread :=
+    @fromStack P (.spawn f bspwn) (.spawn flt bwf)
+
+  namespace WF
+    theorem fromStack!_eq_fromStack {P K} (Kwf : P ⊢ K WF-stack) :
+                                    fromStack! P K = fromStack K Kwf := by
+      simp
+      rw[K.head!_eq_head Kwf.nonnil,
+         getElem!_pos P (K.head Kwf.nonnil).f Kwf.current.flt,
+         getElem!_pos (P[(K.head Kwf.nonnil).f]'Kwf.current.flt) (K.head Kwf.nonnil).b Kwf.current.blt']
+
+    theorem fromStack! {P K} (Pwf : P WF-program) (Kwf : P ⊢ K WF-stack) : P ⊢ fromStack! P K WF-thread :=
+      .mk Kwf (Kwf.code! Pwf)
+
+    theorem fromStack {P K} (Pwf : P WF-program) (Kwf : P ⊢ K WF-stack) : P ⊢ fromStack K Kwf WF-thread :=
+      fromStack!_eq_fromStack Kwf ▸
+      fromStack! Pwf Kwf
+
+    theorem spawn!_eq_spawn {P f bspwn} (flt : f < P.size) (bwf : P[f].B ⊢ bspwn WF-spawn) :
+                            spawn! P f bspwn = spawn P f bspwn flt bwf :=
+      by simp; rw[codeOfGetElem flt bwf.b']
+
+    theorem spawn! {P f bspwn} (Pwf : P WF-program) (flt : f < P.size) (bwf : P[f].B ⊢ bspwn WF-spawn) :
+                   P ⊢ spawn! P f bspwn WF-thread :=
+      fromStack! Pwf (.spawn flt bwf)
+    
+    theorem spawn {P f bspwn} (Pwf : P WF-program) (flt : f < P.size) (bwf : P[f].B ⊢ bspwn WF-spawn) :
+                  P ⊢ spawn P f bspwn flt bwf WF-thread :=
+      fromStack Pwf (.spawn flt bwf)
+  end WF
+end Thread
+
 namespace ThreadTree
   inductive WF (P : Program) : ThreadTree -> Prop where
-    | thread {K} :
-           (Kwf : K.WF P none) ->
-           (thread K).WF P
+    | thread {T} :
+           (Twf : P ⊢ T WF-thread) ->
+           (thread T).WF P
     | node {Rp Rc} :
           (Rpwf : Rp.WF P) ->
           (Rcwf : Rc.WF P) ->
-          (Rp.prom.head? = some (Rc.retjoin P)) ->
+          ((Rp.promsig P).head? = some (Rc.retjoin P)) ->
           (Rc.prom = []) ->
-          (node Rp Rc).WF P
+          (Rp ⋏ Rc).WF P
 
   namespace WF
-    theorem get {P K} : (ThreadTree.thread K).WF P -> K.WF P
-      | thread Kwf => Kwf
-    theorem child {P Rp Rc} : (ThreadTree.node Rp Rc).WF P -> Rc.WF P
+    notation (name := notationwf) P:arg " ⊢ " R " WF-tree" => WF P R
+
+    theorem get {P T} : P ⊢ .thread T WF-tree -> P ⊢ T WF-thread
+      | thread Twf => Twf
+    theorem child {P Rp Rc} : P ⊢ Rp ⋏ Rc WF-tree -> Rc.WF P
       | node _Rpwf Rcwf _Rpprom _Rcprom => Rcwf
-    theorem parent {P Rp Rc} : (ThreadTree.node Rp Rc).WF P -> Rp.WF P
+    theorem parent {P Rp Rc} : (Rp ⋏ Rc).WF P -> Rp.WF P
       | node Rpwf _Rcwf _Rprom _Rcprom => Rpwf
-    theorem parent_prom {P Rp Rc} : (ThreadTree.node Rp Rc).WF P ->
-                                 Rp.prom.head? = some (Rc.retjoin P)
+    theorem parent_prom {P Rp Rc} : (Rp ⋏ Rc).WF P ->
+                                 (Rp.promsig P).head? = some (Rc.retjoin P)
       | node _Rpwf _Rcwf Rpprom _Rcprom => Rpprom
-    theorem child_prom {P Rp Rc} : (ThreadTree.node Rp Rc).WF P -> Rc.prom = []
+    theorem child_prom {P Rp Rc} : (Rp ⋏ Rc).WF P -> Rc.prom = []
       | node _Rpwf _Rcwf _Rpprom Rcprom => Rcprom
 
     instance instDecidable {P} : (R : ThreadTree) -> Decidable (R.WF P)
-      | .thread K => decidable_of_iff (K.WF P none)
+      | .thread T => decidable_of_iff (P ⊢ T WF-thread)
           ⟨thread, λ | thread Kwf => Kwf⟩
-      | .node Rp Rc =>
+      | Rp ⋏ Rc =>
         let _ : Decidable (Rp.WF P) := instDecidable Rp
         let _ : Decidable (Rc.WF P) := instDecidable Rc
         decidable_of_iff (Rp.WF P ∧
                           Rc.WF P ∧
-                          Rp.prom.head? = some (Rc.retjoin P) ∧
+                          (Rp.promsig P).head? = some (Rc.retjoin P) ∧
                           Rc.prom = [])
           ⟨λ ⟨Rwf, Rcwf, Rp, Rcp⟩ => node Rwf Rcwf Rp Rcp,
            λ | node Rwf Rcwf Rp Rcp => ⟨Rwf, Rcwf, Rp, Rcp⟩⟩
+  end WF
 
-    theorem spawn {P f args ret} (Pwf : P.WF) (fwf : SpawnBlock.WF P.fsigs (.mk f args ret)) :
-                  (spawn P f args).WF P := by
-      apply thread
-      apply (.nil ⬝wf ·)
-      exact StackFrame.WF.entry Pwf
-              (by simp; rw[← List.length_map]; exact fwf.flt)
-              (List.getElem_map (α := Func) (·.fsig) ▸
-               (congrArg (α := FuncSig) (·.arity) fwf.sig).symm)
+  @[simp] def spawn (P : Program) (f : FuncIdx) (bspwn : SpawnBlock)
+                    (flt : f < P.size) (bwf : P[f].B ⊢ bspwn WF-spawn) : ThreadTree :=
+    thread (.spawn P f bspwn flt bwf)
 
-    theorem init {P} (Pwf : P.WF) : (ThreadTree.init P).WF P :=
-      spawn (ret := 1) Pwf
-        (.mk Pwf.main_lt
-             (Pwf.head.get0eq ▸ (List.getElem_map (l := P.funs) (·.fsig)).symm))
+  @[simp] def init (P : Program) (Pwf : P WF-program) : ThreadTree :=
+    let main := 0 -- first function in program is main()
+    let entry := SpawnBlock.mk 0 [] -- entry block with no args (since main takes none)
+    let zlt := Pwf.main.zero_lt
+    spawn P main entry zlt (.init Pwf)
+
+  namespace WF
+    theorem spawn!_eq_spawn {P f bspwn} (flt : f < P.size) (bwf : P[f].B ⊢ bspwn WF-spawn) :
+                            spawn! P f bspwn = spawn P f bspwn flt bwf := by
+      simp only [spawn!, spawn]
+      rw[Thread.WF.spawn!_eq_spawn flt bwf]
+    
+    theorem spawn! {P f bspwn} (Pwf : P WF-program) (flt : f < P.size) (bwf : P[f].B ⊢ bspwn WF-spawn) :
+                   P ⊢ spawn! P f bspwn WF-tree :=
+      .thread (.spawn! Pwf flt bwf)
+
+    theorem spawn {P f bspwn} (Pwf : P WF-program) (flt : f < P.size) (bwf : P[f].B ⊢ bspwn WF-spawn) :
+                  P ⊢ spawn P f bspwn flt bwf WF-tree :=
+      .thread (.spawn Pwf flt bwf)
+
+    theorem init!_eq_init {P} (Pwf : P WF-program) : init! P = init P Pwf :=
+      by simp only [init!, init]
+         rw[spawn!_eq_spawn Pwf.main.zero_lt (by simpa using .init Pwf)]
+    
+    theorem init! {P} (Pwf : P WF-program) : P ⊢ init! P WF-tree :=
+      spawn! Pwf Pwf.main.zero_lt (.init Pwf)
+
+    theorem init {P} (Pwf : P WF-program) : P ⊢ init P Pwf WF-tree :=
+      spawn Pwf Pwf.main.zero_lt (.init Pwf)
   end WF
 end ThreadTree
