SporkProofs.lean
@@ -1,6 +1,7 @@
 -- This module serves as the root of the `SporkProofs` library.
 -- Import modules here that should be built as part of the library.
 import SporkProofs.IVec
+import SporkProofs.SimpSet
 import SporkProofs.Syntax
 import SporkProofs.Semantics
 import SporkProofs.ParReduce
