SporkProofs/Preservation.lean
@@ -1,12 +1,15 @@
 import SporkProofs.Syntax
 import SporkProofs.Semantics
+import SporkProofs.WFSyntax
+import SporkProofs.WFSemantics
 
 namespace Step
   theorem preserve_retjoin_stack_cons
-    {P K f ρ₁ ρ₂ X₁ X₂ c₁ c₂} :
+    {P K f ρ₁ ρ₂ X₁ X₂ c₁ c₂}
+    (req : P[f]!.B[c₁]!.r = P[f]!.B[c₂]!.r) :
       CallStack.retjoin P (K ⬝ ⟨f, ρ₁, X₁, c₁⟩) =
       CallStack.retjoin P (K ⬝ ⟨f, ρ₂, X₂, c₂⟩)
-    := by cases K <;> rfl
+    := by simp at req; cases K <;> simp[req]
 
   @[simp] theorem preserve_retjoin_stack_cons_cons {P K k k'} :
       (K ⬝ k ⬝ k').retjoin P = (K ⬝ k).retjoin P :=
@@ -30,63 +33,191 @@ namespace Step
                  preserve_retjoin_stack_append (K' := K')
 
   theorem preserve_retjoin {P : Program} : {R R' : ThreadTree} ->
-                         P ⊢ R ↦ R' -> R.WF P ->
+                         P ⊢ R ↦ R' -> P ⊢ R WF-tree ->
                          R.retjoin P = R'.retjoin P
   | R, R', s => by
-    cases s <;> intro Rwf <;>
-    try (exact preserve_retjoin_stack_cons)
+    cases s <;> intro Rwf
     · case congr_parent Rp Rp' Rc s =>
         simp only [ThreadTree.retjoin]; match Rwf with
           | .node Rpwf Rcwf Rpp Rcp => exact preserve_retjoin s Rpwf
     · case congr_child Rp Rc Rc' s =>
         rfl
-    · case retn f g K ρ' X Y y bret =>
-        exact preserve_retjoin_stack_cons (K := K)
-    · case promote f unpr g prom X K c K' u p =>
-        simp; rw[preserve_retjoin_stack_cons]
+    · case stmt f K ρ X b e v c a =>
+      apply preserve_retjoin_stack_cons
+      rfl
+    · case goto f K ρ X b bnext =>
+      apply preserve_retjoin_stack_cons
+      let flt : f < P.size := Rwf.get.K.current.flt
+      let x := congrArg (·.2) Rwf.get.c.goto_bnext.bsig
+      simp at x
+      rw[getElem!_pos P f flt,
+         getElem!_pos P[f].B bnext.b Rwf.get.c.goto_bnext.blt,
+         getElem!_pos P[f].B b (let y := Rwf.get.K.current.blt
+                                by simp at y; rw[List.length_map]; exact y)]
+      simp; exact x.symm
+    · case ite_true f K ρ X b cond bthen belse n a neq0 =>
+      apply preserve_retjoin_stack_cons
+      let flt := Rwf.get.K.current.flt
+      rw[getElem!_pos P f flt]
+      rw[getElem!_pos P[f].B bthen.b Rwf.get.c.ite_bthen.blt]
+      rw[getElem!_pos P[f].B b (let y := Rwf.get.K.current.blt
+                                by simp at y; rw[List.length_map]; exact y)]
+      exact congrArg (·.2) Rwf.get.c.ite_bthen.bsig.symm
+    · case ite_false f K ρ X b cond bthen belse a =>
+      apply preserve_retjoin_stack_cons
+      let flt := Rwf.get.K.current.flt
+      rw[getElem!_pos P f flt]
+      rw[getElem!_pos P[f].B belse.b Rwf.get.c.ite_belse.blt]
+      rw[getElem!_pos P[f].B b (let y := Rwf.get.K.current.blt
+                                by simp at y; rw[List.length_map]; exact y)]
+      exact congrArg (·.2) Rwf.get.c.ite_belse.bsig.symm
+    · case call f g K ρ b X x bret =>
+      apply preserve_retjoin_stack_cons
+      let flt := Rwf.get.K.current.flt
+      rw[getElem!_pos P f flt]
+      rw[getElem!_pos P[f].B bret.b Rwf.get.c.call_bret.blt]
+      rw[getElem!_pos P[f].B b (let y := Rwf.get.K.current.blt
+                                by simp at y; rw[List.length_map]; exact y)]
+      exact congrArg (·.2) Rwf.get.c.call_bret.bsig.symm
+    · case retn f g K ρ X Y y b bret =>
+      apply preserve_retjoin_stack_cons (K := K)
+      simp
+    · case spork f K ρ X b bbody bspwn =>
+      apply preserve_retjoin_stack_cons
+      let flt := Rwf.get.K.current.flt
+      rw[getElem!_pos P f flt]
+      rw[getElem!_pos P[f].B bbody.b Rwf.get.c.spork_bbody.blt]
+      rw[getElem!_pos P[f].B b (let y := Rwf.get.K.current.blt
+                                by simp at y; rw[List.length_map]; exact y)]
+      exact congrArg (·.2) Rwf.get.c.spork_bbody.bsig.symm
+    · case promote f unpr bspwn prom X K b K' C u p =>
+      let flt := Rwf.get.K.current.flt
+      simp
+      apply preserve_retjoin_stack_cons
+      simp
+    · case spoin_unpr f K ρ bspwn X b bunpr bprom =>
+      apply preserve_retjoin_stack_cons
+      let flt := Rwf.get.K.current.flt
+      rw[getElem!_pos P f flt]
+      rw[getElem!_pos P[f].B bunpr.b Rwf.get.c.spoin_bunpr.blt]
+      rw[getElem!_pos P[f].B b (let y := Rwf.get.K.current.blt
+                                by simp at y; rw[List.length_map]; exact y)]
+      exact congrArg (·.2) Rwf.get.c.spoin_bunpr.bsig.symm
+    · case spoin_prom f g K ρ X b b' bunpr bprom Y y bspwn u =>
+      apply preserve_retjoin_stack_cons
+      let flt := Rwf.parent.get.K.current.flt
+      rw[getElem!_pos P f flt]
+      rw[getElem!_pos P[f].B bprom.b Rwf.parent.get.c.spoin_bprom.blt]
+      rw[getElem!_pos P[f].B b (let y := Rwf.parent.get.K.current.blt
+                                by simp at y; rw[List.length_map]; exact y)]
+      exact congrArg (·.2) Rwf.parent.get.c.spoin_bprom.bsig.symm
+
+    -- · case promote f unpr g prom X K c K' u p =>
+    --     simp; rw[preserve_retjoin_stack_cons]
 
   theorem preserve_prom {P : Program} : {R R' : ThreadTree} ->
-                         P ⊢ R ↦ R' -> R.WF P -> R.prom = R'.prom
+                         P ⊢ R ↦ R' -> P ⊢ R WF-tree -> R.prom = R'.prom
   | R, R', s => by
-    cases s <;> intro Rwf <;> try simp
+    cases s <;> intro Rwf <;> try simp <;> try rfl
     · case congr_parent Rp Rp' Rc Rp_Rp' =>
       rw[preserve_prom Rp_Rp' Rwf.parent]
     · case promote f unpr g prom X K c K' u p =>
       simp[p]
 
+  open CallStack in
+  theorem preserve_promsig {P : Program} : {R R' : ThreadTree} ->
+                            P ⊢ R ↦ R' -> P ⊢ R WF-tree -> R.promsig P = R'.promsig P
+  | R, R', s => by
+    cases s <;> intro Rwf <;> try simp <;> try rfl
+    · case congr_parent Rp Rp' Rc Rp_Rp' =>
+      rw[preserve_promsig Rp_Rp' Rwf.parent]
+    · case promote f unpr bspwn prom X K b K' c u p =>
+      simp[CallStack.prom_promsig_nil.mp p]
+
   
   open ThreadTree.WF (thread node) in
-  theorem preservation {P : Program} (Pwf : P.WF) :
+  theorem preservation {P : Program} (Pwf : P WF-program) :
                        {R R' : ThreadTree} ->
-                       R.WF P -> P ⊢ R ↦ R' -> R'.WF P := by
+                       P ⊢ R WF-tree -> P ⊢ R ↦ R' -> P ⊢ R' WF-tree := by
     intro R R' wf R_R'; cases R_R' <;> cases wf
 
     · case congr_parent Rp Rp' Rc Rp_Rp' Rpwf Rcwf Rcp Rpp =>
-        exact node (preservation Pwf Rpwf Rp_Rp') Rcwf (preserve_prom Rp_Rp' Rpwf ▸ Rpp) Rcp
+        exact node (preservation Pwf Rpwf Rp_Rp') Rcwf (preserve_promsig Rp_Rp' Rpwf ▸ Rpp) Rcp
 
     · case congr_child Rp Rc Rc' Rc_Rc' Rpwf Rcwf Rcp Rpp =>
         exact node Rpwf (preservation Pwf Rcwf Rc_Rc')
                         (preserve_retjoin Rc_Rc' Rcwf ▸ Rpp)
                         (preserve_prom Rc_Rc' Rcwf ▸ Rcp)
 
-    · case stmt f K ρ X e v c a wf =>
+    · case stmt f K ρ X b e v c a wf =>
         apply thread
         exact match wf with
-           | Kwf ⬝wf (.mk p ρwf _ (.code (.stmt ewf cwf))) =>
-             Kwf ⬝wf (.mk p ρwf rfl (.code
-                 (by simp[BlockSig.bind] at cwf; simp; exact cwf)))
+           | .mk (Kwf ⬝wf (.mk flt blt bsig ρwf)) (.stmt ewf cwf) =>
+             let flt : f < P.size := wf.K.current.flt
+             .mk (Kwf ⬝wf (.mk (X := X.concat v) flt blt
+                    ⟨by simp; simp at bsig;
+                        exact Nat.le_trans bsig.1 (Nat.le_add_right X.length 1), bsig.2⟩
+                    ρwf))
+             --(.mk bwf.blt bwf.bsig (bwf.args.map (λ x xwf => by simp; exact xwf.weaken)))
+                 (by simp[BlockSig.bind] at cwf; simp; exact cwf)
 
-    · case goto f K ρ X bnext wf =>
+    · case goto f K ρ X b bnext wf =>
         apply thread
         exact match wf with
-          | Kwf ⬝wf (.mk p ρwf _ (.code (.goto bnext_wf)))=>
-            Kwf ⬝wf (.goto Pwf p ρwf bnext_wf)
+          | .mk (Kwf ⬝wf (.mk flt blt bsig ρwf)) (.goto bnext_wf) =>
+              by simp only [getters] at bnext_wf; exact
+              .mk ((by simp only[StackFrame.ret, getters, CallStack.bsig] at Kwf bsig bnext_wf
+                       simp only[StackFrame.ret, getters]
+                       rw[bnext_wf.bsig]
+                       exact Kwf) ⬝wf
+                   (.mk flt bnext_wf.blt ⟨bnext_wf.bsig ▸
+                                          by simp;
+                                             let x := argsOfGetElem bnext_wf.args
+                                             simp at x
+                                             rw[x, X.getElem_length bnext_wf.args]
+                                             exact Nat.le_refl bnext.args.length,
+                                          bsig.2 ▸ congrArg (·.σ) bnext_wf.bsig ▸
+                                          by simp only [getters, CallStack.bsig, bsig.2]⟩ ρwf))
+                  (by simp only [CallStack.bsig, getters]
+                      let p := wf.c.goto_bnext.bsig
+                      simp only [Thread.K, CallStack.head, StackFrame.f] at p
+                      let bnextlt : bnext.b < P[f].B.length :=
+                        by simp; rw[← List.length_map Block.bsig]; exact bnext_wf.blt
+                      let bnextlt_wf : bnext.b < P[f].size :=
+                        by simpa using wf.c.goto_bnext.blt
+                      let cwf := Pwf⁅f⁆⁅bnext.b⁆.code
+                      simp only [getters] at cwf
+                      simp only [← getElem!_pos P[f].B bnext.b bnextlt] at p cwf ⊢
+                      simp only [← getElem!_pos P f flt] at p cwf ⊢
+                      simp at cwf
+                      rw[p]
+                      simp only [getElem!_pos P f flt] at p cwf ⊢
+                      simp only [getElem!_pos P[f].B bnext.b bnextlt] at p cwf ⊢
+                      simp only [getters, CallStack.bsig, ← bsig.2]
+                      simp only [getElem!_pos P[f] bnext.b bnextlt_wf]
+                      let cwf₂ : P.fsigs; P[f].B; P[f].B[bnext.b] ⊢ P[f][bnext.b].code WF-code :=
+                        by simp; exact cwf
+                      let xpf : X[bnext.args]!.length = P[f].B[bnext.b].Γ :=
+                        argsOfGetElem bnext_wf.args ▸
+                        ValMap.getElem_length bnext_wf.args ▸
+                        (congrArg BlockSig.Γ bnext_wf.bsig).symm
+                      rw[xpf]
+                      rw[← @BlockSig.get_fix P[f].B[bnext.b]] at cwf₂
+                      let rpf := congrArg BlockSig.r wf.c.goto_bnext.bsig
+                      let σpf := congrArg BlockSig.σ wf.c.goto_bnext.bsig
+                      let σpf' : P[f].B[b].σ = SpawnDeque.sig P[f].B ρ :=
+                        wf.K.current.bsig.2
+                      simp only [getters, CallStack.bsig] at rpf σpf
+                      rw[← rpf, σpf']
+                      rw[σpf] at cwf₂
+                      exact cwf₂)
 
     · case ite_true f K ρ X cond bthen belse n cond_n neq0 wf =>
         apply thread
         exact match wf with
-          | Kwf ⬝wf (.mk p ρwf _ (.code (.ite cond_wf bthen_wf belse_wf))) =>
-            Kwf ⬝wf (.goto Pwf p ρwf bthen_wf)
+          | .mk (Kwf ⬝wf (.mk flt blt bsig ρwf)) (.ite cond_wf bthen_wf belse_wf) =>
+            .mk (Kwf ⬝wf (.mk sorry sorry sorry sorry))
+                (.goto Pwf p ρwf bthen_wf)
 
     · case ite_false f K ρ X cond bthen belse cond_0 wf =>
         apply thread
@@ -140,9 +271,9 @@ namespace Step
     · case promote f unpr g prom X K c K' u p wf =>
         let kProm := CallStack.allPromoted_iff_nil.mpr u
         let rec hp : {K' : CallStack} -> {gets : Option Nat} -> K'.prom = [] ->
-                     CallStack.WF P gets (K ⬝ ⟨f, ⟨g :: unpr, prom⟩, X, c⟩ ++ K') ->
-                     CallStack.WF P gets (K ⬝ ⟨f, ⟨unpr, g.ret :: prom⟩, X, c⟩ ++ K') ∧
-                     CallStack.WF P none {⟨g.f, ∅, g.args, .codeEntry P g.f⟩} ∧
+                     P; gets ⊢ (K ⬝ ⟨f, ⟨g :: unpr, prom⟩, X, c⟩ ++ K') WF-stack ->
+                     P; gets ⊢ (K ⬝ ⟨f, ⟨unpr, g.ret :: prom⟩, X, c⟩ ++ K') WF-stack ∧
+                     P; none ⊢ {⟨g.f, ∅, g.args, .codeEntry P g.f⟩} WF-stack ∧
                      g.ret = P[g.f]!.fsig.ret
           | .nil, gets, _, wf => by
             rw[CallStack.append_nil] at *
