SporkProofs/Progress.lean
@@ -1,68 +1,66 @@
 import SporkProofs.Syntax
 import SporkProofs.Semantics
+import SporkProofs.WFSyntax
+import SporkProofs.WFSemantics
 
 namespace Step
 
   inductive Next (P : Program) : ThreadTree -> Type where
-    | result (g X x) :
-        Next P {{⟨g, ∅, X, .code (.retn x)⟩}}
-    | blocked (K f gret π X bunpr bprom) :
-        Next P {K ⬝ ⟨f, ⟨[], gret :: π⟩, X, .code (.spoin bunpr bprom)⟩}
+    | result (f X b x) :
+        Next P {{⟨f, ∅, X, b⟩} ⋄ (.retn x)}
+    | blocked (K f bspwn π X b bunpr bprom) :
+        Next P {K ⬝ ⟨f, ⟨[], bspwn :: π⟩, X, b⟩ ⋄ (.spoin bunpr bprom)}
     | step {R} (R') (s : P ⊢ R ↦ R') :
         Next P R
   
   def progress {P : Program} :
-               (R : ThreadTree) -> R.WF P ->
+               (R : ThreadTree) -> P ⊢ R WF-tree ->
                Next P R
     | .node Rp Rc, wf =>
-      let Rpwf : Rp.WF P := wf.parent
+      let Rpwf : P ⊢ Rp WF-tree := wf.parent
       let Rcwf := wf.child
       match progress Rp Rpwf with
-        | .result g X x =>
+        | .result g X b x =>
           nomatch wf.parent_prom
         | .step Rp' s =>
           .step _ (congr_parent s)
-        | .blocked K f gret π X bunpr bprom =>
+        | .blocked K f bspwn π X b bunpr bprom =>
           let Rpb : ThreadTree :=
-            {K ⬝ ⟨f, ⟨[], gret :: π⟩, X, .code (.spoin bunpr bprom)⟩}
-          let Rpbwf : Rpb.WF P := wf.parent
+            {K ⬝ ⟨f, ⟨[], bspwn :: π⟩, X, b⟩ ⋄ (.spoin bunpr bprom)}
+          let Rpbwf : P ⊢ Rpb WF-tree := wf.parent
           match progress Rc Rcwf with
-            | .result g Y y =>
-              .step _ (.spoin_prom (g := ⟨g, default /- doesn't matter -/, gret⟩)
-                         (K.allPromoted_iff_nil.mp
-                           (wf.parent.get.head.ρwf.prom.prom_canProm_true
-                             K.allPromoted)))
-            | .blocked K' f' gret' π' X' bunpr' bprom' =>
+            | .result g Y b' y =>
+              .step _ (.spoin_prom (K.allPromoted_iff_nil.mp
+                  (wf.parent.get.K.head.ρwf.prom.prom_canProm_true K.allPromoted)))
+            | .blocked K' f' gret' π' X' b' bunpr' bprom' =>
               nomatch wf.child_prom
             | .step Rc' s =>
               .step _ (congr_child s)
-    | .thread (K ⬝ ⟨f, ρ, X, .code (.stmt e c)⟩), wf =>
-      .step _ (.stmt (.mk wf.get.head.cwf.c.stmt_expr))
-    | .thread (K ⬝ ⟨f, ρ, X, .code (.goto bnext)⟩), wf =>
+    | .thread (K ⬝ ⟨f, ρ, X, b⟩ ⋄ (.stmt e c)), wf =>
+      .step _ (.stmt (.mk wf.get.c.stmt_expr))
+    | .thread (K ⬝ ⟨f, ρ, X, b⟩ ⋄ (.goto bnext)), wf =>
       .step _ .goto
-    | .thread (K ⬝ ⟨f, ρ, X, .code (.ite cond bthen belse)⟩), wf =>
-      if p : cond.eval X wf.get.head.cwf.c.ite_cond = 0 then
-        .step _ (.ite_false (p ▸ .mk wf.get.head.cwf.c.ite_cond))
+    | .thread (K ⬝ ⟨f, ρ, X, b⟩ ⋄ (.ite cond bthen belse)), wf =>
+      if p : cond.eval X wf.get.c.ite_cond = 0 then
+        .step _ (.ite_false (p ▸ .mk wf.get.c.ite_cond))
       else
-        .step _ (.ite_true (.mk wf.get.head.cwf.c.ite_cond) p)
-    | .thread (K ⬝ ⟨f, ρ, X, .code (.call g args bret)⟩), wf =>
+        .step _ (.ite_true (.mk wf.get.c.ite_cond) p)
+    | .thread (K ⬝ ⟨f, ρ, X, b⟩ ⋄ (.call g args bret)), wf =>
       .step _ .call
-    | .thread (K ⬝ ⟨f, ρ, X, .cont bnext⟩ ⬝ ⟨g, ρempty, Y, .code (.retn y)⟩), wf =>
+    | .thread (K ⬝ ⟨f, ρ, X, bret⟩ ⬝ ⟨g, ρempty, Y, b⟩ ⋄ (.retn y)), wf =>
       let p : ρempty = ∅ :=
-        by cases ρempty <;> cases wf.get.head.cwf.c <;> simp_all; rfl
+        by cases ρempty <;> cases wf.get.c <;> simp_all; rfl
       p ▸ .step _ .retn
-    | .thread (K ⬝ ⟨f, ρ, X, .code c⟩ ⬝ ⟨g, ρempty, Y, .code (.retn y)⟩), wf =>
-      nomatch wf.get.tail.head.isCont
-    | .thread (.nil ⬝ ⟨g, ρempty, Y, .code (.retn y)⟩), wf =>
+    | .thread (.nil ⬝ ⟨g, ρempty, Y, b⟩ ⋄ (.retn y)), wf =>
       let p : ρempty = ∅ :=
-        by cases ρempty <;> cases wf.get.head.cwf.c <;> simp_all; rfl
-      p ▸ .result g Y y
-    | .thread (K ⬝ ⟨f, ρ, X, .code (.spork bbody g args)⟩), wf =>
+        by cases ρempty <;> cases wf.get.c <;> simp_all; rfl
+      p ▸ .result g Y b y
+    | .thread (K ⬝ ⟨f, ρ, X, b⟩ ⋄ (.spork bbody bspwn)), wf =>
       .step _ .spork
-    | .thread (K ⬝ ⟨f, ρ, X, .code (.spoin bunpr bprom)⟩), wf =>
+    | .thread (K ⬝ ⟨f, ρ, X, b⟩ ⋄ (.spoin bunpr bprom)), wf =>
       match ρ with
         | ⟨[], []⟩ =>
-          nomatch wf.get.head.cwf.c.spoin_sn_nonnil
+          nomatch wf.get.c.spoin_oblg
         | ⟨u :: us, ps⟩ =>
           let sc := (u :: us).getLast (by simp)
           let us' := (u :: us).dropLast
@@ -70,5 +68,5 @@ namespace Step
             by simp; symm; exact (u :: us).dropLast_concat_getLast (by simp)
           pf ▸ .step _ .spoin_unpr
         | ⟨[], p :: ps⟩ =>
-          .blocked _ _ _ _ _ _ _
+          .blocked _ _ _ _ _ _ _ _
 end Step
