SporkProofs/SimpSet.lean
@@ -1,0 +1,2 @@
+import Lean
+register_simp_attr getters
